{
 "cells": [
  {
   "cell_type": "markdown",
   "id": "188d623d-79cb-4d7e-aaed-112bb84d8d33",
   "metadata": {},
   "source": [
    "$\\textbf{Assignment}$\n",
    "Instructions:\n",
    "- Use latex.\n",
    "- Write your latex in jupyter notebook.\n",
    "- Push your answer to your github account.\n",
    "- Deadline is 2 weeks before finals.\n",
    "- Fail to submit 2 weeks before finals is an automatic 5.0 for this assignment.\n",
    "- Each problem is 25 points.\n",
    "\n",
    "1. Recall the definition of a rational number, denoted as $\\mathbb{Q}$. Prove that the Euler's number $e = \\Sigma_{k=0}^\\infty \\frac{1}{k!} \\notin \\mathbb{Q}$. A factorial is defined as $k! = (k)(k-1)(k-2)(k-3)..., \\forall k \\in \\mathbb{Z}^+$, note that $0! = 1$. Furthermore, a sum notation $\\Sigma_{k=0}^\\infty k = 0+ 1 + 2 + 3 +....+...$\n",
    "e, \\( e \\notin \\mathbb{Q} \\).\n",
    "2. Prove Minkowski's Inequality for sums, $\\forall \\ p>1, (a_k, b_k)>0$:\n",
    "\\begin{gather}\n",
    "\\begin{bmatrix}\n",
    "\\Sigma_{k=1}^n |a_k + b_k|^p\n",
    "\\end{bmatrix}^\\frac{1}{p}\n",
    "\\leq\n",
    "\\begin{bmatrix}\n",
    "\\Sigma_{k=1}^n |a_k|^p\n",
    "\\end{bmatrix}^\\frac{1}{p}\n",
    "+\n",
    "\\begin{bmatrix}\n",
    "\\Sigma_{k=1}^n |b_k|^p\n",
    "\\end{bmatrix}^\\frac{1}{p}\n",
    "\\end{gather}\n",
    "\n",
    "3. Prove the triangle inequality $|x+y| \\leq |x| + |y|, \\forall (x,y) \\in \\mathbb{R}$\n",
    "\n",
    "4. Prove Sedrakayan's Lemma $\\forall u_i, v_i \\in \\mathbb{R}^+$:\n",
    "\\begin{gather}\n",
    "\\frac{(\\Sigma_{i=1}^n u_i)^2}{\\Sigma_{i=1}^n v_i}\n",
    "\\leq\n",
    "\\Sigma_{i=1}^n \\frac{(u_i)^2}{v_i}\n",
    "\\end{gather}"
   ]
  },
  {
   "cell_type": "markdown",
   "id": "1de33a92-7a6a-4624-a8c5-994644cffc20",
   "metadata": {},
   "source": [
    "1. Consider the functions $f(x) = 2x+1$, $g(x)=2y-1$, $j(x) = |f(x)+g(x)|$, and $h(x) = j(x)^2$, show for the following inequality that:\n",
    "\n",
    "\\begin{gather}\n",
    "\\sqrt{|f(x)|^2} \\geq \\sqrt{h(x)} - \\sqrt{|g(x)|^2}, \\forall (x,y) \\in \\mathbb{Z}^+\n",
    "\\end{gather}"
   ]
  },
  {
   "cell_type": "markdown",
   "id": "997eb723-4112-443b-92d6-4f6734ea8e3b",
   "metadata": {},
   "source": [
    "2. Prove Sedrakayan's Lemma if $u_i, v_i$ are square roots of an even integers:\n",
    "\\begin{gather}\n",
    "\\frac{(\\Sigma_{i=1}^n u_i)^2}{\\Sigma_{i=1}^n v_i}\n",
    "\\leq\n",
    "\\Sigma_{i=1}^n \\frac{(u_i)^2}{v_i}\n",
    "\\end{gather}"
   ]
  },
  {
   "cell_type": "markdown",
   "id": "feac60fb-0599-4bad-89a7-a7d503348696",
   "metadata": {},
   "source": [
    "To demonstrate that Euler's number $e = \\sum_{k=0}^\\infty \\frac{1}{k!} \\notin \\mathbb{Q}$, we aim to establish a proof.\n",
    "\n",
    "$\\textit{Proof:}$\n",
    "\n",
    "Let's assume, for contradiction, that $e$ can be expressed as a rational number, i.e., $e = \\frac{a}{b}$, where $a$ and $b$ are integers and $b \\neq 0$.\n",
    "\n",
    "We can represent the series expansion of $e$ as:\n",
    "\n",
    "$e = \\sum_{k=0}^\\infty \\frac{1}{k!} = 1 + \\frac{1}{1!} + \\frac{1}{2!} + \\frac{1}{3!} + \\dots $\n",
    "\n",
    "Multiplying both sides by $b!$ to eliminate the denominators, we get:\n",
    "\n",
    "$b!e = b!\\left(1 + \\frac{1}{1!} + \\frac{1}{2!} + \\frac{1}{3!} + \\dots \\right) = b!(1 + b + \\frac{b(b-1)}{2!} + \\frac{b(b-1)(b-2)}{3!} + \\dots)$\n",
    "\n",
    "Observing that every term on the right side is an integer multiple of $b!$, it follows that $e$ should also be rational. This conclusion contradicts our initial assumption. Thus, $e \\notin \\mathbb{Q}$.\n"
   ]
  },
  {
   "cell_type": "markdown",
   "id": "a093a6f7-723e-4d75-b69c-ca63750a4eb1",
   "metadata": {},
   "source": [
    "To prove Minkowski's Inequality for sums:\n",
    " $\\left(\\sum_{k=1}^n |a_k + b_k|^p\\right)^\\frac{1}{p} \\leq \\left(\\sum_{k=1}^n |a_k|^p\\right)^\\frac{1}{p} + \\left(\\sum_{k=1}^n |b_k|^p\\right)^\\frac{1}{p} $\n",
    "\n",
    "$\\textit{Proof:}$\n",
    "\n",
    "It involves using Hölder's inequality. Let $q$ be the conjugate exponent of $p$ (i.e., $\\frac{1}{p} + \\frac{1}{q} = 1$).\n",
    "\n",
    "Applying Hölder's inequality with $p$ and $q$ to the sequences $(|a_k|^p)$ and $(1)$, and to the sequences $(|b_k|^p)$ and $(1)$:\n",
    "\n",
    " $\\sum_{k=1}^n |a_k|^p \\cdot 1 \\leq \\left(\\sum_{k=1}^n |a_k|^p\\right)^\\frac{1}{p} \\left(\\sum_{k=1}^n 1^q\\right)^\\frac{1}{q} = \\left(\\sum_{k=1}^n |a_k|^p\\right)^\\frac{1}{p} \\cdot n^\\frac{1}{q} $\n",
    " $\\sum_{k=1}^n |b_k|^p \\cdot 1 \\leq \\left(\\sum_{k=1}^n |b_k|^p\\right)^\\frac{1}{p} \\left(\\sum_{k=1}^n 1^q\\right)^\\frac{1}{q} = \\left(\\sum_{k=1}^n |b_k|^p\\right)^\\frac{1}{p} \\cdot n^\\frac{1}{q} $\n",
    "\n",
    "And then Add these inequalities:\n",
    "\n",
    " $\\sum_{k=1}^n |a_k|^p + \\sum_{k=1}^n |b_k|^p \\leq \\left(\\sum_{k=1}^n |a_k|^p\\right)^\\frac{1}{p} \\cdot n^\\frac{1}{q} + \\left(\\sum_{k=1}^n |b_k|^p\\right)^\\frac{1}{p} \\cdot n^\\frac{1}{q} $\n",
    "\n",
    " $\\sum_{k=1}^n (|a_k|^p + |b_k|^p) \\leq \\left(\\sum_{k=1}^n |a_k|^p\\right)^\\frac{1}{p} \\cdot n^\\frac{1}{q} + \\left(\\sum_{k=1}^n |b_k|^p\\right)^\\frac{1}{p} \\cdot n^\\frac{1}{q} $\n",
    "\n",
    "Now raising both sides to the power of $\\frac{1}{p}$:\n",
    "\n",
    " $\\left(\\sum_{k=1}^n (|a_k|^p + |b_k|^p)\\right)^\\frac{1}{p} \\leq \\left(\\left(\\sum_{k=1}^n |a_k|^p\\right)^\\frac{1}{p} \\cdot n^\\frac{1}{q} + \\left(\\sum_{k=1}^n |b_k|^p\\right)^\\frac{1}{p} \\cdot n^\\frac{1}{q}\\right)^\\frac{1}{p} $\n",
    "\n",
    " $\\left(\\sum_{k=1}^n (|a_k + b_k|^p)\\right)^\\frac{1}{p} \\leq \\left(\\sum_{k=1}^n |a_k|^p\\right)^\\frac{1}{p} + \\left(\\sum_{k=1}^n |b_k|^p\\right)^\\frac{1}{p} $\n",
    "\n",
    "Which successfully proves Minkowski's Inequality.\n"
   ]
  },
  {
   "cell_type": "markdown",
   "id": "a775d915-9bf5-4aee-8964-df61ff9605ce",
   "metadata": {},
   "source": [
    "\n",
    "$\\textit{Proof:}$\n",
    "\n",
    "Let's analyze three scenarios:\n",
    "\n",
    "When both $x$ and $y$ are non-negative ($x \\geq 0$ and $y \\geq 0$), we have $|x| = x$ and $|y| = y$, resulting in $|x+y| = x+y$. Consequently, $|x+y| = x + y \\leq |x| + |y|$.\n",
    "When $x$ is non-negative and $y$ is negative ($x \\geq 0$ and $y < 0$), we get $|x| = x$ and $|y| = -y$, leading to $|x+y| = x-y$. In this case, $|x+y| = x - y \\leq |x| + |y|$.\n",
    "When both $x$ and $y$ are negative ($x < 0$ and $y < 0$), we find $|x| = -x$ and $|y| = -y$, yielding $|x+y| = -(x+y) = -x - y$. Thus, $|x+y| = -(x + y) \\leq |x| + |y|$."
   ]
  },
  {
   "cell_type": "markdown",
   "id": "c9ce9dd4-6134-488c-ae0e-673e4136e7c4",
   "metadata": {},
   "source": [
    "Prove Sedrakayan's Lemma $\\forall u_i, v_i \\in \\mathbb{R}^+$:\n",
    "\n",
    "$\\frac{(\\sum_{i=1}^n u_i)^2}{\\sum_{i=1}^n v_i} \\leq \\sum_{i=1}^n \\frac{(u_i)^2}{v_i}$\n",
    "\n",
    "$\\textit{Proof:}$\n",
    "\n",
    "Let $\\mathbf{u} = (u_1, u_2, ..., u_n)$ and $\\mathbf{v} = (v_1, v_2, ..., v_n)$ be vectors in $\\mathbb{R}^+$.\n",
    "\n",
    "By Cauchy-Schwarz Inequality, we have:\n",
    "\n",
    "$\\left(\\sum_{i=1}^n u_i v_i\\right)^2 \\leq \\left(\\sum_{i=1}^n u_i^2\\right) \\left(\\sum_{i=1}^n v_i^2\\right)$\n",
    "\n",
    "Since $v_i > 0$ for all $i$, we can divide both sides by $\\left(\\sum_{i=1}^n v_i^2\\right): \\frac{\\left(\\sum_{i=1}^n u_i v_i\\right)^2}{\\left(\\sum_{i=1}^n v_i^2\\right)} \\leq \\sum_{i=1}^n u_i^2$\n",
    "\n",
    "Now, notice that $\\left(\\sum_{i=1}^n u_i v_i\\right) = \\mathbf{u} \\cdot \\mathbf{v}$ and $\\sum_{i=1}^n u_i^2 = \\|\\mathbf{u}\\|^2$, where $\\|\\cdot\\|$ denotes the Euclidean norm.\n",
    "\n",
    "Thus, we have: $\\frac{(\\mathbf{u} \\cdot \\mathbf{v})^2}{\\|\\mathbf{v}\\|^2} \\leq \\|\\mathbf{u}\\|^2$\n",
    "\n",
    "Dividing both sides by $\\|\\mathbf{v}\\|^2$, we get: $\\frac{(\\mathbf{u} \\cdot \\mathbf{v})^2}{\\|\\mathbf{v}\\|^2 \\|\\mathbf{v}\\|^2} \\leq \\frac{\\|\\mathbf{u}\\|^2}{\\|\\mathbf{v}\\|^2}$\n",
    "\n",
    "Simplifying, we obtain: $\\frac{(\\mathbf{u} \\cdot \\mathbf{v})^2}{\\|\\mathbf{v}\\|^4} \\leq \\frac{\\|\\mathbf{u}\\|^2}{\\|\\mathbf{v}\\|^2}$\n",
    "\n",
    "Now, substituting $\\|\\mathbf{v}\\|^2 = \\sum_{i=1}^n v_i$ and rearranging, we get: $\\frac{(\\sum_{i=1}^n u_i)^2}{\\sum_{i=1}^n v_i} \\leq \\sum_{i=1}^n \\frac{u_i^2}{v_i}$\n",
    "\n",
    "Proving Sedrakayan's Lemma."
   ]
  },
  {
   "cell_type": "markdown",
   "id": "0e12787a-f3a7-4abf-b22d-9c34f0864239",
   "metadata": {},
   "source": [
    "$\\textit{Proof:}$\n",
    "\n",
    "First, let's express $f(x)$, $g(x)$, and $h(x)$ in terms of $x$ and $y$:\n",
    "\n",
    "$f(x) = 2x + 1$\n",
    "\n",
    "$g(x) = 2y - 1$\n",
    "\n",
    "$j(x) = |f(x) + g(x)| = |(2x + 1) + (2y - 1)| = |2x + 2y| = 2|x + y|$\n",
    "\n",
    "$h(x) = j(x)^2 = (2|x + y|)^2 = 4|x + y|^2$\n",
    "\n",
    "Now, let's substitute $f(x)$, $g(x)$, and $h(x)$ back into the inequality:\n",
    "\n",
    "$\\sqrt{|(2x + 1)|^2} \\geq \\sqrt{(4|x + y|^2)} - \\sqrt{|(2y - 1)|^2}$\n",
    "\n",
    "Simplify each term:\n",
    "\n",
    "$\\sqrt{(2x + 1)^2} \\geq \\sqrt{4(|x + y|^2)} - \\sqrt{(2y - 1)^2}$\n",
    "\n",
    "$|2x + 1| \\geq 2|x + y| - |2y - 1|$\n",
    "\n",
    "Now, let's consider the absolute value expressions:\n",
    "\n",
    "1. $|2x + 1| = \\begin{cases} 2x + 1, & \\text{if } 2x + 1 \\geq 0 \\\\ -(2x + 1), & \\text{if } 2x + 1 < 0 \\end{cases}$\n",
    "2. $|2y - 1| = \\begin{cases} 2y - 1, & \\text{if } 2y - 1 \\geq 0 \\\\ -(2y - 1), & \\text{if } 2y - 1 < 0 \\end{cases}$\n",
    "\n",
    "Given that $x$ and $y$ are positive integers, both $2x + 1$ and $2y - 1$ are non-negative.\n",
    "\n",
    "Substitute back into the inequality:\n",
    "\n",
    "$2x + 1 \\geq 2|x + y| - (2y - 1)$\n",
    "\n",
    "$2x + 1 \\geq 2x + 2y - 2y + 1$\n",
    "\n",
    "$2x + 1 \\geq 2x + 1$\n",
    "\n",
    "This inequality holds true for all positive integers $x$ and $y$. Therefore, the inequality is true.\n",
    "\n",
    "We have shown that: $\\sqrt{|f(x)|^2} \\geq \\sqrt{h(x)} - \\sqrt{|g(x)|^2}, \\forall (x,y) \\in \\mathbb{Z}^+$"
   ]
  },
  {
   "cell_type": "markdown",
   "id": "815e3690-b3f4-4d8f-b1a9-1d05664f7d31",
   "metadata": {},
   "source": [
    "$\\textit{Proof:}$\n",
    "\n",
    "Let $u_i = \\sqrt{2x_i}$ and $v_i = \\sqrt{2y_i}$, where $x_i$ and $y_i$ are positive integers.\n",
    "\n",
    "Substitute $u_i$ and $v_i$ into the inequality:\n",
    "\n",
    "$\\frac{\\left(\\sum_{i=1}^n \\sqrt{2x_i}\\right)^2}{\\sum_{i=1}^n \\sqrt{2y_i}} \\leq \\sum_{i=1}^n \\frac{(\\sqrt{2x_i})^2}{\\sqrt{2y_i}}$\n",
    "\n",
    "$\\frac{\\left(\\sum_{i=1}^n \\sqrt{2x_i}\\right)^2}{\\sum_{i=1}^n \\sqrt{2y_i}} \\leq \\sum_{i=1}^n \\frac{2x_i}{\\sqrt{2y_i}}$\n",
    "\n",
    "Now, let's show that for any positive real numbers $a_i$ and $b_i$, we have:\n",
    "\n",
    "$\\left(\\sum_{i=1}^n a_i\\right)^2 \\leq n \\sum_{i=1}^n b_i$\n",
    "\n",
    "This is equivalent to:\n",
    "\n",
    "$\\left(\\sum_{i=1}^n a_i\\right)^2 \\leq \\sum_{i=1}^n (b_i)^2$\n",
    "\n",
    "which is a well-known result from the Cauchy-Schwarz Inequality.\n",
    "\n",
    "Substitute $a_i = \\sqrt{2x_i}$ and $b_i = \\frac{\\sqrt{2y_i}}{\\sqrt{n}}$ into the inequality:\n",
    "\n",
    "$\\left(\\sum_{i=1}^n \\sqrt{2x_i}\\right)^2 \\leq n \\sum_{i=1}^n \\left(\\frac{\\sqrt{2y_i}}{\\sqrt{n}}\\right)^2$\n",
    "\n",
    "$\\left(\\sum_{i=1}^n \\sqrt{2x_i}\\right)^2 \\leq \\sum_{i=1}^n 2y_i$\n",
    "\n",
    "Now, let's substitute this result back into our inequality:\n",
    "\n",
    "$\\frac{\\left(\\sum_{i=1}^n \\sqrt{2x_i}\\right)^2}{\\sum_{i=1}^n \\sqrt{2y_i}} \\leq \\sum_{i=1}^n \\frac{2x_i}{\\sqrt{2y_i}}$\n",
    "\n",
    "$\\frac{\\sum_{i=1}^n 2x_i}{\\sum_{i=1}^n \\sqrt{2y_i}} \\leq \\sum_{i=1}^n \\frac{2x_i}{\\sqrt{2y_i}}$\n",
    "\n",
    "$\\frac{\\sum_{i=1}^n 2x_i}{\\sum_{i=1}^n \\sqrt{2y_i}} \\leq \\sum_{i=1}^n \\frac{2x_i}{\\sqrt{2y_i}}$\n",
    "\n",
    "Since both sides are non-negative, we can square both sides of the inequality:\n",
    "\n",
    "$\\left(\\frac{\\sum_{i=1}^n 2x_i}{\\sum_{i=1}^n \\sqrt{2y_i}}\\right)^2 \\leq \\left(\\sum_{i=1}^n \\frac{2x_i}{\\sqrt{2y_i}}\\right)^2$\n",
    "\n",
    "$\\frac{\\left(\\sum_{i=1}^n 2x_i\\right)^2}{\\left(\\sum_{i=1}^n \\sqrt{2y_i}\\right)^2} \\leq \\sum_{i=1}^n \\frac{4x_i^2}{2y_i}$\n",
    "\n",
    "$\\frac{\\left(\\sum_{i=1}^n 2x_i\\right)^2}{\\sum_{i=1}^n 2y_i} \\leq \\sum_{i=1}^n \\frac{2x_i^2}{y_i}$\n",
    "\n",
    "$\\frac{\\left(\\sum_{i=1}^n u_i\\right)^2}{\\sum_{i=1}^n v_i} \\leq \\sum_{i=1}^n \\frac{(u_i)^2}{v_i}$\n",
    "\n",
    "Proving Sedrakayan's Lemma when $u_i$ and $v_i$ are square roots of even integers.\n"
   ]
  },
  {
   "cell_type": "code",
   "execution_count": null,
   "id": "cdd83210-68c6-423a-8ed5-935049d88d04",
   "metadata": {},
   "outputs": [],
   "source": []
  }
 ],
 "metadata": {
  "kernelspec": {
   "display_name": "Python 3 (ipykernel)",
   "language": "python",
   "name": "python3"
  },
  "language_info": {
   "codemirror_mode": {
    "name": "ipython",
    "version": 3
   },
   "file_extension": ".py",
   "mimetype": "text/x-python",
   "name": "python",
   "nbconvert_exporter": "python",
   "pygments_lexer": "ipython3",
   "version": "3.11.7"
  }
 },
 "nbformat": 4,
 "nbformat_minor": 5
}
